rocq-brick-libstdcpp/proof/mutex/spec/lock_guard.v
@@ -92,14 +92,14 @@ Section with_cpp.
     \pre mutex.not_locked g thr qt
     \post
       this |-> R (mp, g, q, qt) 1$m P **
-      P ** mutex.locked g thr qt
+      P ** mutex.locked g (Some thr) qt
     ).
 
   cpp.spec "std::lock_guard<std::mutex>::~lock_guard()" as dtor_spec from source with (
     \this this
     \pre{mp g q qt P} this |-> R (mp, g, q, qt) 1$m P
     \persist{thr} current_thread thr
-    \pre mutex.locked g thr qt
+    \pre mutex.locked g (Some thr) qt
     \pre ▷P
     \post
       mutex.not_locked g thr qt **
