rocq-brick-libstdcpp/proof/mutex/spec/scoped_lock.v
@@ -35,8 +35,8 @@ Module scoped_lock.
         \pre mutex.not_locked g2 thr qt2
         \post
           this |-> R 1$m [ (mp1, g1, q1, qt1, P1); (mp2, g2, q2, qt2, P2)] **
-          P1 ** mutex.locked g1 thr qt1 **
-          P2 ** mutex.locked g2 thr qt2
+          P1 ** mutex.locked g1 (Some thr) qt1 **
+          P2 ** mutex.locked g2 (Some thr) qt2
       ).
 
       cpp.spec "std::scoped_lock<...<std::mutex, std::mutex>>::~scoped_lock()"
@@ -51,8 +51,8 @@ Module scoped_lock.
           this |-> R 1$m [ (mp1, g1, q1, qt1, P1); (mp2, g2, q2, qt2, P2)]
         \pre |> P1
         \pre |> P2
-        \pre mutex.locked g1 thr qt1
-        \pre mutex.locked g2 thr qt2
+        \pre mutex.locked g1 (Some thr) qt1
+        \pre mutex.locked g2 (Some thr) qt2
         \post
           mp1 |-> mutex.R g1 q1$m P1 ** mutex.not_locked g1 thr qt1 **
           mp2 |-> mutex.R g2 q2$m P2 ** mutex.not_locked g2 thr qt2
